code/bignum/Hacl.Spec.Bignum.Exponentiation.fsti
@@ -7,8 +7,42 @@ open Lib.Sequence
 
 open Hacl.Spec.Bignum.Definitions
 
+module BM = Hacl.Spec.Bignum.Montgomery
 
 #reset-options "--z3rlimit 50 --fuel 0 --ifuel 0"
+
+
+let bn_mod_exp_pre
+  (#nLen:size_pos{128 * nLen <= max_size_t})
+  (n:lbignum nLen)
+  (a:lbignum nLen)
+  (bBits:size_pos)
+  (b:lbignum (blocks bBits 64))
+ =
+   bn_v n % 2 = 1 /\ 1 < bn_v n /\
+   0 < bn_v b /\ bn_v b < pow2 bBits /\ bn_v a < bn_v n
+
+
+let bn_mod_exp_post
+  (#nLen:size_pos{128 * nLen <= max_size_t})
+  (n:lbignum nLen)
+  (a:lbignum nLen)
+  (bBits:size_pos)
+  (b:lbignum (blocks bBits 64))
+  (res:lbignum nLen)
+ =
+  bn_mod_exp_pre n a bBits b /\
+  bn_v res == Lib.NatMod.pow_mod #(bn_v n) (bn_v a) (bn_v b)
+
+
+val check_mod_exp:
+    #nLen:size_pos{128 * nLen <= max_size_t}
+  -> n:lbignum nLen
+  -> a:lbignum nLen
+  -> bBits:size_pos
+  -> b:lbignum (blocks bBits 64) ->
+  res:bool{res <==> bn_mod_exp_pre n a bBits b}
+
 
 // This function is *NOT* constant-time on the exponent b
 val bn_mod_exp_precompr2:
@@ -29,11 +63,10 @@ val bn_mod_exp_precompr2_lemma:
   -> b:lbignum (blocks bBits 64)
   -> r2:lbignum nLen -> Lemma
   (requires
-    bn_v n % 2 = 1 /\ 1 < bn_v n /\ bn_v n < pow2 (64 * nLen) /\
-    0 < bn_v b /\ bn_v b < pow2 bBits /\ bn_v a < bn_v n /\
+    bn_mod_exp_pre n a bBits b /\
     bn_v r2 == pow2 (128 * nLen) % bn_v n)
   (ensures
-    bn_v (bn_mod_exp_precompr2 nLen n a bBits b r2) == Lib.NatMod.pow_mod #(bn_v n) (bn_v a) (bn_v b))
+    bn_mod_exp_post n a bBits b (bn_mod_exp_precompr2 nLen n a bBits b r2))
 
 
 // This function is constant-time on the exponent b
@@ -55,11 +88,10 @@ val bn_mod_exp_mont_ladder_precompr2_lemma:
   -> b:lbignum (blocks bBits 64)
   -> r2:lbignum nLen -> Lemma
   (requires
-    bn_v n % 2 = 1 /\ 1 < bn_v n /\ bn_v n < pow2 (64 * nLen) /\
-    0 < bn_v b /\ bn_v b < pow2 bBits /\ bn_v a < bn_v n /\
+    bn_mod_exp_pre n a bBits b /\
     bn_v r2 == pow2 (128 * nLen) % bn_v n)
   (ensures
-    bn_v (bn_mod_exp_mont_ladder_precompr2 nLen n a bBits b r2) == Lib.NatMod.pow_mod #(bn_v n) (bn_v a) (bn_v b))
+    bn_mod_exp_post n a bBits b (bn_mod_exp_mont_ladder_precompr2 nLen n a bBits b r2))
 
 
 // This function is *NOT* constant-time on the exponent b
@@ -78,11 +110,8 @@ val bn_mod_exp_lemma:
   -> a:lbignum nLen
   -> bBits:size_pos
   -> b:lbignum (blocks bBits 64) -> Lemma
-  (requires
-    bn_v n % 2 = 1 /\ 1 < bn_v n /\ bn_v n < pow2 (64 * nLen) /\
-    0 < bn_v b /\ bn_v b < pow2 bBits /\ bn_v a < bn_v n)
-  (ensures
-    bn_v (bn_mod_exp nLen n a bBits b) == Lib.NatMod.pow_mod #(bn_v n) (bn_v a) (bn_v b))
+  (requires bn_mod_exp_pre n a bBits b)
+  (ensures  bn_mod_exp_post n a bBits b (bn_mod_exp nLen n a bBits b))
 
 
 // This function is constant-time on the exponent b
@@ -101,8 +130,5 @@ val bn_mod_exp_mont_ladder_lemma:
   -> a:lbignum nLen
   -> bBits:size_pos
   -> b:lbignum (blocks bBits 64) -> Lemma
-  (requires
-    bn_v n % 2 = 1 /\ 1 < bn_v n /\ bn_v n < pow2 (64 * nLen) /\
-    0 < bn_v b /\ bn_v b < pow2 bBits /\ bn_v a < bn_v n)
-  (ensures
-    bn_v (bn_mod_exp_mont_ladder nLen n a bBits b) == Lib.NatMod.pow_mod #(bn_v n) (bn_v a) (bn_v b))
+  (requires bn_mod_exp_pre n a bBits b)
+  (ensures  bn_mod_exp_post n a bBits b (bn_mod_exp_mont_ladder nLen n a bBits b))
